Worked on proof of soundness for loop

src/E3_sound.thy
@@ -64,15 +64,28 @@ where "wf_ct_nt_items_for_nt f \<equiv> \<forall>n ntitem s i j as. ntitem \<in>
 (ntitem = (n, [], (NT n) # as, i, i))"  
 
 definition wf_item_ops :: "'string ty_ops \<Rightarrow> bool"
-where "wf_item_ops tyops \<equiv> \<forall>sym i j nt as bs j'. sym_dot_i9 tyops (sym, i, j) = i \<and> sym_dot_j9 tyops (sym, i, j) = j \<and> sym6 tyops (sym, i, j) = sym \<and> with_j9 tyops (nt,as,bs,i,j) j'= (nt,as,bs,i,j') \<and> shift_a2_b2_c2 tyops (nt,as,bs,i,j) = (nt,(hd bs) # as, tl bs, i, j)"
+where "wf_item_ops tyops \<equiv> \<forall>sym i j nt as bs j'. sym_dot_i9 tyops (sym, i, j) = i \<and> sym_dot_j9 tyops (sym, i, j) = j \<and> sym6 tyops (sym, i, j) = sym \<and> with_j9 tyops (nt,as,bs,i,j) j'= (nt,as,bs,i,j') \<and> shift_a2_b2_c2 tyops (nt,as,bs,i,j) = (nt,(hd bs) # as, tl bs, i, j) \<and> mk_item tyops = id"
 
 definition impl_maps :: "'string ty_impl_ctxt \<Rightarrow> bool"
 where "impl_maps ctxt \<equiv> maps ctxt = impl_ctxt_map"
 
-lemma t: "wf_item_ops (item_ops5 ctxt) \<Longrightarrow> impl_maps ctxt \<Longrightarrow> (sym1, as, bs, i, j) \<in> blocked5 s0 k \<Longrightarrow> NTITM (sym1, (hd bs) # as, tl bs, i, j) \<in> (set (todo5 (Finite_Set.fold (\<lambda>bitm. \<lambda>x. E3.cut ctxt bitm citm x) (s0\<lparr>todo5 := list\<rparr>) (blocked5 s0 k))))  "
+lemma cut_todo: "sets ctxt = impl_ctxt_set \<Longrightarrow> wf_item_ops (item_ops5 ctxt) \<Longrightarrow> E3.cut ctxt (sym1, as, bs, i, j) (sym2, i2, j2) s0 = s1 \<Longrightarrow> ( NTITM (sym1, (hd bs) # as, tl bs, i, j2) \<notin> todo_done5 s0 \<and> todo5 s1 = (NTITM (sym1, (hd bs) # as, tl bs, i, j2)) # (todo5 s0)) \<or> (NTITM (sym1, (hd bs) # as, tl bs, i, j2) \<in> todo_done5 s0 \<and> s0 = s1)"
+apply(unfold E3.cut_def add_todo_def impl_ctxt_set_def impl_std_def wf_item_ops_def)
+apply(simp add: Let_def rev_apply_def wf_item_ops_def )
+apply(case_tac "NTITM (sym1, (hd bs) # as, tl bs, i, j2) \<in> todo_done5 s0")
+apply(clarsimp)
+apply(force)
+done
+
+lemma t: "sets ctxt = impl_ctxt_set \<Longrightarrow> wf_item_ops (item_ops5 ctxt) \<Longrightarrow>  impl_maps ctxt \<Longrightarrow> (sym1, as, bs, i, j) \<in> blocked5 s0 (i', sym2) \<Longrightarrow>(Finite_Set.fold (\<lambda>bitm. \<lambda>x. E3.cut ctxt bitm (sym2, i', j') x) (s0) (blocked5 s0 (i', sym2))) = s1 \<Longrightarrow> NTITM (sym1, (hd bs) # as, tl bs, i, j') \<in> set (todo5 s1) \<or> NTITM (sym1, (hd bs) # as, tl bs, i, j') \<in> todo_done5 s0"
 apply(unfold E3.cut_def wf_item_ops_def impl_maps_def)
 apply(simp add: Let_def rev_apply_def)
-apply(unfold impl_ctxt_map_def add_todo_def)
+apply(unfold impl_ctxt_map_def add_todo_def impl_ctxt_set_def impl_std_def impl_mbk_def)
+apply(clarsimp)
+apply(unfold Finite_Set.fold_def)
+apply(unfold fold_graph_def)
+apply(clarsimp)
+
 
 
 lemma sound_init: "wf_ct_nt_items_for_nt (ct_nt_items_for_nt ps) \<Longrightarrow> loop2_inv s ps (init_state s ps)"
@@ -89,19 +102,15 @@ lemma sound: "wf_ct_nt_items_for_nt (ct_nt_items_for_nt ps) \<Longrightarrow> wf
   apply(unfold loop2_def loop2_inv_def)
   apply(simp add: rev_apply_def Let_def)
   apply(unfold pop_todo_def)
-  apply(case_tac "todo5 s0")
+  apply(induct "todo5 s0")
   apply(simp_all)
   apply(case_tac "dest_item (item_ops5 ctxt) a")
-  apply(simp)
   apply(case_tac  "b2_nil (item_ops5 ctxt) prod")
-  apply(simp)
   apply(case_tac "mk_sym_coord (item_ops5 ctxt) (nt2 (item_ops5 ctxt) prod, nt_dot_i9 (item_ops5 ctxt) prod, nt_dot_j9 (item_ops5 ctxt) prod)")
-  apply(simp)
   apply(unfold wf_item_ops_def)
   apply(simp add: rev_apply_def)
   apply(unfold impl_maps_def)
   apply(unfold impl_ctxt_map_def)
-  apply(simp)
   apply(unfold impl_mbk_def)
   apply(simp)
   apply(unfold impl_mck_def)
